dimsum_examples/rec.v
@@ -2103,6 +2103,21 @@ Proof.
   - erewrite map_difference_eq_dom_L => //. apply _.
 Qed.
 
+(** ** Properties of rec_link *)
+Lemma asm_link_comm fns1 fns2 m1 m2 :
+  fns1 ## fns2 →
+  trefines (rec_link fns1 fns2 m1 m2)
+           (rec_link fns2 fns1 m2 m1).
+Proof.
+  move => ?. unshelve apply: link_comm. {
+    exact (λ _ s1 s2, s2 = (λ o : seq_product_case, sp_opp <$> o) <$> s1). }
+  - move => /= p s e p' s' e' ok s2 HR1 ?. destruct!/=. split!.
+    case_match; destruct!/=; split!; repeat case_bool_decide => //=.
+    1: set_solver.
+    all: try destruct p as [[]|]; try destruct p' as [[]|]; naive_solver.
+  - done.
+Qed.
+
 (** ** Commuting and associativity of semantic linking (WIP) *)
 (*
 (* TODO: track a stack of this and compute every thing from it (also keep an optional event) *)
